tzimtzum/Tzimtzum/Soundness/PresMost.lean
@@ -13,68 +13,81 @@ set_option linter.unreachableTactic false
 
 namespace Tzimtzum
 
+variable {AgentId ToolId InvocationId CapKind EgressKind IssuerId InstructionId : Type}
+
 /-! ## Initiation -/
 
-theorem init_sound (s : KSt) (hi : initial s) : allInv s := by
+theorem init_sound (s : St AgentId ToolId InvocationId CapKind EgressKind IssuerId InstructionId)
+    (hi : initial s) : allInv s := by
   kav_discharge initial
 
 /-! ## Per-action preservation (cascade) -/
 
-theorem pres_register_tool (s s' : KSt) (hinv : allInv s)
+theorem pres_register_tool (s s' : St AgentId ToolId InvocationId CapKind EgressKind IssuerId InstructionId)
+    (hinv : allInv s)
     (hn : (Kav.close1 register_tool).next s s') : allInv s' := by
   simp only [Kav.close1] at hn
   obtain ⟨tool, hg, hn⟩ := hn
   kav_discharge register_tool
 
-theorem pres_load_instruction (s s' : KSt) (hinv : allInv s)
+theorem pres_load_instruction (s s' : St AgentId ToolId InvocationId CapKind EgressKind IssuerId InstructionId)
+    (hinv : allInv s)
     (hn : (Kav.close2 load_instruction).next s s') : allInv s' := by
   simp only [Kav.close2] at hn
   obtain ⟨a, instr, hg, hn⟩ := hn
   kav_discharge load_instruction
 
-theorem pres_delegate (s s' : KSt) (hinv : allInv s)
+theorem pres_delegate (s s' : St AgentId ToolId InvocationId CapKind EgressKind IssuerId InstructionId)
+    (hinv : allInv s)
     (hn : (Kav.close2 delegate).next s s') : allInv s' := by
   simp only [Kav.close2] at hn
   obtain ⟨grantor, grantee, hg, hn⟩ := hn
   kav_discharge delegate
 
-theorem pres_grant_capability (s s' : KSt) (hinv : allInv s)
+theorem pres_grant_capability (s s' : St AgentId ToolId InvocationId CapKind EgressKind IssuerId InstructionId)
+    (hinv : allInv s)
     (hn : (Kav.close3 grant_capability).next s s') : allInv s' := by
   simp only [Kav.close3] at hn
   obtain ⟨prnt, child, cap, hg, hn⟩ := hn
   kav_discharge grant_capability
 
-theorem pres_revoke (s s' : KSt) (hinv : allInv s)
+theorem pres_revoke (s s' : St AgentId ToolId InvocationId CapKind EgressKind IssuerId InstructionId)
+    (hinv : allInv s)
     (hn : (Kav.close2 revoke).next s s') : allInv s' := by
   simp only [Kav.close2] at hn
   obtain ⟨prnt, target, hg, hn⟩ := hn
   kav_discharge revoke
 
-theorem pres_cascade_revoke (s s' : KSt) (hinv : allInv s)
+theorem pres_cascade_revoke (s s' : St AgentId ToolId InvocationId CapKind EgressKind IssuerId InstructionId)
+    (hinv : allInv s)
     (hn : (Kav.close2 cascade_revoke).next s s') : allInv s' := by
   simp only [Kav.close2] at hn
   obtain ⟨child, prnt, hg, hn⟩ := hn
   kav_discharge cascade_revoke
 
-theorem pres_invoke_start (s s' : KSt) (hinv : allInv s)
+theorem pres_invoke_start (s s' : St AgentId ToolId InvocationId CapKind EgressKind IssuerId InstructionId)
+    (hinv : allInv s)
     (hn : (Kav.close3 invoke_start).next s s') : allInv s' := by
   simp only [Kav.close3] at hn
   obtain ⟨a, tool, inv, hg, hn⟩ := hn
   kav_discharge invoke_start
 
-theorem pres_return_unendorsed (s s' : KSt) (hinv : allInv s)
+theorem pres_return_unendorsed (s s' : St AgentId ToolId InvocationId CapKind EgressKind IssuerId InstructionId)
+    (hinv : allInv s)
     (hn : (Kav.close2 return_unendorsed).next s s') : allInv s' := by
   simp only [Kav.close2] at hn
   obtain ⟨child, prnt, hg, hn⟩ := hn
   kav_discharge return_unendorsed
 
-theorem pres_sentinel_elevate_taint (s s' : KSt) (hinv : allInv s)
+theorem pres_sentinel_elevate_taint (s s' : St AgentId ToolId InvocationId CapKind EgressKind IssuerId InstructionId)
+    (hinv : allInv s)
     (hn : (Kav.close2 sentinel_elevate_taint).next s s') : allInv s' := by
   simp only [Kav.close2] at hn
   obtain ⟨a, l, hg, hn⟩ := hn
   kav_discharge sentinel_elevate_taint
 
-theorem pres_sentinel_refresh_budget (s s' : KSt) (hinv : allInv s)
+theorem pres_sentinel_refresh_budget (s s' : St AgentId ToolId InvocationId CapKind EgressKind IssuerId InstructionId)
+    (hinv : allInv s)
     (hn : (Kav.close1 sentinel_refresh_budget).next s s') : allInv s' := by
   simp only [Kav.close1] at hn
   obtain ⟨a, hg, hn⟩ := hn
